\section{Задние}

Доказать что:
\begin{equation}
    A^i_{\ ;i} = \cfrac{1}{\sqrt{-g}} \piv{}{x^i}\inner{\sqrt{-g} A^i}
\end{equation}

Справа получим:

\begin{equation}
    \piv{}{x^i}\inner{\sqrt{-g} A^i} = 
    \piv{\sqrt{-g}}{x^i}A^i + \sqrt{-g}\piv{A^i}{x^i} = 
    -\cfrac{1}{2\sqrt{-g}} \piv{g}{x^i}A^i + \sqrt{-g}\piv{A^i}{x^i} =
    \cfrac{gg_{jk}g^{jk}_{\ \ ,i}}{2\sqrt{-g}} A^i + \sqrt{-g}\piv{A^i}{x^i}
\end{equation}

Слева распишем по определению:
\begin{equation}
    A^i_{\ ;i} = \piv{A^i}{x^i} + \Gamma^j_{\ lj} A^{l} 
\end{equation}


Седеним и сократим что можем:
\begin{equation}
    \piv{A^i}{x^i} + \Gamma^j_{\ lj} A^{l} = 
    \cfrac{1}{\cancel{\sqrt{-g}}} \cfrac{\cancel{g}g_{jk}g^{jk}_{\ \ ,i}}{2\cancel{\sqrt{-g}}} A^i 
    + \cfrac{\sqrt{-g}}{\cancel{\sqrt{-g}}} \piv{A^i}{x^i}
    =\cfrac{1}{2} g_{jk}g^{jk}_{\ \ ,i} A^i + \piv{A^i}{x^i}
\end{equation}

\begin{equation}
    \label{eq_1}
    \cancel{\piv{A^i}{x^i}} + \Gamma^j_{\ lj} A^{l} = 
    \cfrac{1}{2} g_{jk}g^{jk}_{\ \ ,i} A^i + \cancel{\piv{A^i}{x^i}}
\end{equation}

Теперь поиграемся:

\begin{equation}
    \Gamma_{ijk} + \Gamma_{jik} = \crist{i}{j}{k} + \crist{j}{i}{k} = g_{ij,k}
\end{equation}

\begin{equation}
    g^{ij}_{\ \ ,k} = -\inner{\Gamma_{lnk} + \Gamma_{nlk}} g^{nj} g^{li}
\end{equation}

\begin{equation}
    \label{eq_2}
    g_{jk}g^{jk}_{\ \ ,i} = -\inner{\Gamma_{lni} + \Gamma_{nli}} g^{nk} g^{lj }g_{jk} = -\inner{\Gamma_{lni} + \Gamma_{nli}} g^{nl} = 2 \Gamma^l_{\ li} = 2 \Gamma^l_{\ il}
\end{equation}

Подставляем в \ref{eq_1} и получем верное тождество.


